LiveVerif/src/LiveVerifExamples/network.v
@@ -1,0 +1,128 @@
+(* -*- eval: (load-file "../LiveVerif/live_verif_setup.el"); -*- *)
+Require Import LiveVerif.LiveVerifLib.
+Require Import bedrock2.TraceInspection.
+Require Import bedrock2.NetworkPackets.
+Require Import LiveVerifExamples.mbuf.
+Require Import LiveVerifExamples.e1000.
+
+Require Import coqutil.Map.OfListWord.
+
+Load LiveVerif.
+
+
+(* should high-level trace be packets expressed as list of bytes
+   or as memory chunks? *)
+
+Definition concat_preds(P Q: list byte -> Prop): list byte -> Prop :=
+  fun bs => exists bs1 bs2, bs = bs1 ++ bs2 /\ P bs1 /\ Q bs2.
+
+Definition pure_pred(P: Prop): list byte -> Prop := fun bs => bs = nil /\ P.
+
+Definition and_preds(P Q: list byte -> Prop): list byte -> Prop :=
+  fun bs => P bs /\ Q bs.
+
+Definition has_len(n: Z): list byte -> Prop := fun bs => len bs = n.
+
+Definition any: list byte -> Prop := fun _ => True.
+
+Definition eqZs(zs: list Z): list byte -> Prop :=
+  fun bs => List.map byte.unsigned bs = zs.
+
+Definition mbuf(payload: list byte -> Prop): list byte -> Prop :=
+  and_preds (has_len MBUF_SIZE) (concat_preds payload any).
+
+(*
+Definition mbuf(n: Z)(bs: list Z): list byte -> Prop :=
+  and_preds (has_len MBUF_SIZE) (concat_preds (and_preds (has_len n) (eqZs bs)) any).
+*)
+
+Definition eth_header_bytes(h: ethernet_header_t): list byte -> Prop. Admitted.
+Definition ip_header_bytes(h: ip_header_t): list byte -> Prop. Admitted.
+Definition udp_header_bytes(h: udp_header_t): list byte -> Prop. Admitted.
+
+Definition eth_buf(h: ethernet_header_t)(payload: list byte -> Prop): list byte -> Prop :=
+  mbuf (concat_preds (eth_header_bytes h) payload).
+
+Definition ip_buf(eh: ethernet_header_t)(ih: ip_header_t)
+  (payload: list byte -> Prop): list byte -> Prop :=
+  eth_buf eh (concat_preds (ip_header_bytes ih) payload).
+
+Definition udp_buf(eh: ethernet_header_t)(ih: ip_header_t)(uh: udp_header_t)
+  (payload: list byte -> Prop): list byte -> Prop :=
+  ip_buf eh ih (concat_preds (udp_header_bytes uh) payload).
+
+(*
+Definition eth_buf(h: ethernet_header_t)(n: Z)(bs: list Z): word -> mem -> Prop :=
+  exists header_bytes, decode_ethernet_header header_bytes = h /\
+  mbuf (sizeof ethernet_header + n) (header_bytes ++ bs)
+
+  <{ * ethernet_header h a
+     * array (uint 8) n bs (a ^+ /[sizeof ethernet_header])
+     * array (uint 8) (MBUF_SIZE - n - sizeof ethernet_header) ?
+         (a ^+ /[sizeof ethernet_header + n]) }>.
+
+Definition eth_buf(h: ethernet_header_t)(n: Z)(bs: list Z)(a: word): mem -> Prop :=
+  <{ * ethernet_header h a
+     * array (uint 8) n bs (a ^+ /[sizeof ethernet_header])
+     * array (uint 8) (MBUF_SIZE - n - sizeof ethernet_header) ?
+         (a ^+ /[sizeof ethernet_header + n]) }>.
+ TODO define using mbuf? *)
+
+Definition bytes_pred_at(P: list byte -> Prop)(a: word)(m: mem): Prop :=
+  exists bs, m = map.of_list_word_at a bs /\ P bs.
+
+Definition eth_buff(h: ethernet_header_t)(n: Z)(zs: list Z): word -> mem -> Prop :=
+  bytes_pred_at (eth_buf h (and_preds (has_len n) (eqZs zs))).
+
+Axiom network: word -> mem -> Prop. (* TODO takes more params *)
+
+(** * Alloc/free packets, bottom-up: *)
+
+Instance spec_of_net_alloc_eth: fnspec :=                                          .**/
+
+uintptr_t net_alloc_eth(uintptr_t nw) /**#
+  ghost_args := (R: mem -> Prop);
+  requires t m := <{ * network nw
+                     * R }> m;
+  ensures t' m' r := t' = t /\ exists h,
+       <{ * network nw
+          * eth_buff h 0 nil r
+          * R }> m' #**/                                                   /**.
+
+
+(** * Transmit, bottom-up: *)
+
+(* net_tx_eth *)
+
+(* net_tx_ip *)
+
+Instance spec_of_net_tx_udp: fnspec :=                                          .**/
+
+void net_tx_udp(uintptr_t nw, uintptr_t b, uintptr_t n) /**#
+  ghost_args := bs (R: mem -> Prop);
+  requires t m := <{ * mbuf.mbuf \[n] bs b (* TODO udp_buf *)
+                     * R }> m;
+  (* rx may change the mbuf arbitrarily, but must return it *)
+  ensures t' m' := t' = t /\
+       <{ * R * R }> m' #**/                                                   /**.
+
+
+(** * Receive, top-down: *)
+
+(* net_rx_udp *)
+
+(* net_rx_ip *)
+
+Instance spec_of_net_rx_eth: fnspec :=                                          .**/
+
+void net_rx_eth(uintptr_t a, uintptr_t n) /**#
+  ghost_args := bs (R: mem -> Prop);
+  requires t m := <{ * mbuf.mbuf \[n] bs a
+                     * R }> m;
+  (* rx may change the mbuf arbitrarily, but must return it *)
+  ensures t' m' := t' = t /\ exists bs' n',
+       <{ * mbuf.mbuf n' bs' a
+          * R }> m' #**/                                                   /**.
+
+
+End LiveVerif. Comments .**/ //.
